WIP

security/BacktranslationProof2.v
@@ -620,6 +620,23 @@ Section PROOFGENV.
     rewrite ! Genv.genv_pol_add_globals. ss.
   Qed.
 
+  Lemma gen_program_match_symbs
+        p_a btr
+        p_c ge_a ge_c
+        (P_C: p_c = gen_program btr p_a)
+        (GE_A: ge_a = Genv.globalenv p_a)
+        (GE_C: ge_c = globalenv p_c)
+        (WFPP: wf_program_public p_a)
+        (NR: list_norepet (prog_defs_names p_a))
+    :
+    match_symbs ge_a ge_c.
+  Proof.
+    unfold match_symbs. splits.
+    eapply gen_program_symbs_public; eauto.
+    eapply gen_program_symbs_find; eauto.
+    eapply gen_program_symbs_volatile; eauto.
+  Qed.
+
   Lemma gen_program_match_genv
         p_a btr
         p_c ge_a ge_c
@@ -631,10 +648,7 @@ Section PROOFGENV.
     :
     match_genv ge_a ge_c.
   Proof.
-    unfold match_genv, match_symbs. splits.
-    eapply gen_program_symbs_public; eauto.
-    eapply gen_program_symbs_find; eauto.
-    eapply gen_program_symbs_volatile; eauto.
+    unfold match_genv. splits. eapply gen_program_match_symbs; eauto.
     eapply gen_program_eq_policy; eauto.
   Qed.
 
@@ -646,7 +660,7 @@ Section PROOFINIT.
   Lemma gen_counter_defs_alloc
         x0 gds cnts
         (CNTS: cnts = gen_counter_defs x0 gds)
-        (ge: genv)
+        F V (ge: Genv.t F V)
     :
     Forall (fun (idg: ident * (globdef fundef type)) =>
               let (_, y) := idg in
@@ -770,6 +784,26 @@ Section PROOFINIT.
     }
   Qed.
 
+  Lemma genv_alloc_globals_exists
+        ge
+        gds
+        (FA: Forall (fun (idg: ident * (globdef fundef type)) =>
+                       let (_, y) := idg in
+                       match y with
+                       | Gfun _ => True
+                       | Gvar v =>
+                           Genv.init_data_list_aligned 0 (gvar_init v) /\
+                             (forall (i : ident) (o : ptrofs), In (Init_addrof i o) (gvar_init v) -> exists b : block, Genv.find_symbol ge i = Some b)
+                       end) gds)
+        m
+    :
+    exists m', Genv.alloc_globals ge m gds = Some m'.
+  Proof.
+    revert_until FA. induction FA; i; ss. eauto.
+    hexploit Genv.alloc_global_exists. eapply H. intros (m' & ALLOC).
+    rewrite ALLOC. eauto.
+  Qed.
+
   Lemma gen_program_exists_init_mem
         btr (p: Asm.program)
         m_a
@@ -782,130 +816,51 @@ Section PROOFINIT.
     hexploit gen_program_exists_init_mem_1; auto. eauto. apply MEMA.
     intros ALLOC1. erewrite <- Genv.alloc_globals_app.
     2:{ apply ALLOC1. }
+    eapply genv_alloc_globals_exists. eapply Forall_impl. 2: eapply gen_counter_defs_alloc; eauto.
+    i. destruct a as (ida & gda). des_ifs. des. splits; eauto.
+  Qed.
 
-    TODO
+  Lemma gen_program_prog_main_eq
+        p btr
+    :
+    prog_main (gen_program btr p) = AST.prog_main p.
+  Proof. ss. Qed.
 
-
-Genv.alloc_global_exists:
-  forall [F V : Type] {CF : has_comp F} (ge : Genv.t F V) (m : mem) (idg : ident * globdef F V),
-  (let (_, y) := idg in
-   match y with
-   | Gfun _ => True
-   | Gvar v =>
-       Genv.init_data_list_aligned 0 (gvar_init v) /\
-       (forall (i : ident) (o : ptrofs), In (Init_addrof i o) (gvar_init v) -> exists b : block, Genv.find_symbol ge i = Some b)
-   end) -> exists m' : mem, Genv.alloc_global ge m idg = Some m'
-
-  Definition wf_c_state (ge: Clight.genv) (tr ttr: bundle_trace) (cnts: cnt_ids) id (cst: Clight.state) :=
-    match cst with
-    | State f stmt k_c e le m_c =>
-        wf_counters ge m_c tr cnts /\
-          ( (wf_c_nb ge m_c))
-    | _ => False
-    end.
-(forall (id : ident) (b : block) (f : function),
- Genv.find_symbol ge id = Some b ->
- Genv.find_funct_ptr ge b = Some (Internal f) ->
- exists cnt : ident,
-   cnts ! id = Some cnt /\ wf_counter ge m (comp_of f) (Datatypes.length (get_id_tr tr id)) cnt)
-     : genv -> mem -> bundle_trace -> cnt_ids -> Prop
-  Definition match_state (ge_i: Asm.genv) (ge_c: Clight.genv) (k: meminj) tr cnts pars id (ist: ir_state) (cst: Clight.state) :=
-    match ist, cst with
-    | Some (cur, m_i, k_i), State f _ k_c e le m_c =>
-        (match_genv ge_i ge_c) /\ (match_mem ge_i k m_i m_c) /\
-          (match_cur_fun ge_i ge_c cur f id) /\ (match_find_def ge_i ge_c cnts pars tr) /\
-          (match_cont ge_c tr cnts k_c k_i) /\
-          (match_params pars ge_c ge_i) /\
-          (match_cnts cnts ge_c k)
-    | _, _ => False
-    end.
-
-Genv.alloc_globals = 
-fun (F V : Type) (CF : has_comp F) (ge : Genv.t F V) =>
-fix alloc_globals (m : mem) (gl : list (ident * globdef F V)) {struct gl} : option mem :=
-  match gl with
-  | [] => Some m
-  | g :: gl' => match Genv.alloc_global ge m g with
-                | Some m' => alloc_globals m' gl'
-                | None => None
-                end
-  end
-      : forall F V : Type, has_comp F -> Genv.t F V -> mem -> list (ident * globdef F V) -> option mem
-
-Genv.alloc_globals_app:
-  forall [F V : Type] {CF : has_comp F} (ge : Genv.t F V) (gl1 gl2 : list (ident * globdef F V)) (m : mem) [m1 : mem],
-  Genv.alloc_globals ge m gl1 = Some m1 -> Genv.alloc_globals ge m1 gl2 = Genv.alloc_globals ge m (gl1 ++ gl2)
-
-Genv.init_mem = 
-fun (F V : Type) (CF : has_comp F) (p : AST.program F V) => Genv.alloc_globals (Genv.globalenv p) Mem.empty (AST.prog_defs p)
-     : forall F V : Type, has_comp F -> AST.program F V -> option mem
-
-Genv.globals_initialized = 
-fun (F V : Type) (ge g : Genv.t F V) (m : mem) =>
-forall (b : block) (gd : globdef F V),
-Genv.find_def g b = Some gd ->
-match gd with
-| Gfun _ =>
-    Mem.perm m b 0 Cur Nonempty /\
-    (forall (ofs : Z) (k : perm_kind) (p : permission), Mem.perm m b ofs k p -> ofs = 0 /\ p = Nonempty)
-| Gvar v =>
-    Mem.range_perm m b 0 (init_data_list_size (gvar_init v)) Cur (Genv.perm_globvar v) /\
-    (forall (ofs : Z) (k : perm_kind) (p : permission),
-     Mem.perm m b ofs k p -> 0 <= ofs < init_data_list_size (gvar_init v) /\ perm_order (Genv.perm_globvar v) p) /\
-    (gvar_volatile v = false -> Genv.load_store_init_data ge m b 0 (gvar_init v) (Some (gvar_comp v))) /\
-    (gvar_volatile v = false ->
-     Mem.loadbytes m b 0 (init_data_list_size (gvar_init v)) (Some (gvar_comp v)) =
-     Some (Genv.bytes_of_init_data_list ge (gvar_init v)))
-end
-     : forall F V : Type, Genv.t F V -> Genv.t F V -> mem -> Prop
-wf_counter = 
-fun (ge : Senv.t) (m : mem) (cp : compartment) (n : nat) (cnt : ident) =>
-Senv.public_symbol ge cnt = false /\
-(exists b : block,
-   Senv.find_symbol ge cnt = Some b /\
-   Mem.valid_access m Mint64 b 0 Writable (Some cp) /\
-   Mem.loadv Mint64 m (Vptr b Ptrofs.zero) (Some cp) = Some (Vlong (nat64 n)))
-     : Senv.t -> mem -> compartment -> nat -> ident -> Prop
+  Lemma exists_initial_state
+        p ist
+        (INIT: ir_initial_state p ist)
+        (WFMAINSIG: wf_main_sig p)
+        (NR: list_norepet (map fst (AST.prog_defs p)))
+        btr
+    :
+    exists f m_c, initial_state (gen_program btr p) (Callstate (Internal f) [] Kstop m_c)
+             /\
+               ((fn_params f = []) /\ (fn_vars f = []) /\ (fn_temps f = [])).
+  Proof.
+    inv INIT. des. hexploit gen_program_exists_init_mem; eauto. intros (m_c & INIT_MC).
+    hexploit gen_program_match_find_def; eauto. intros MFD. unfold match_find_def in MFD.
+    ss. hexploit Genv.find_invert_symbol. eapply H. intros INV_A.
+    specialize (WFMAINSIG _ _ H H0).
+    rewrite Genv.find_funct_ptr_iff in H0. specialize (MFD _ _ _ H0 INV_A).
+    des_ifs. ss. rewrite <- Genv.find_funct_ptr_iff in MFD.
+    assert (l = []).
+    { hexploit in_gds_exists_params.
+      { eapply PTree_Properties.of_list_norepet. eauto. apply in_prog_defmap.
+        rewrite Genv.find_def_symbol. exists cur. splits; eauto.
+      }
+      auto.
+      intros. des. rewrite Heq0 in H2. clarify. ss. rewrite WFMAINSIG in *. ss.
+      symmetry in H4. apply map_eq_nil in H4. subst. ss.
+    }
+    subst. do 2 eexists. split.
+    - econs; eauto.
+      (* exists (Callstate (Internal (gen_function (Genv.globalenv p) i l (get_id_tr btr (AST.prog_main p)) f)) nil Kstop m_c). econs; eauto. *)
+      { rewrite gen_program_prog_main_eq. eapply gen_program_symbs_find in H; ss; eauto. apply H. }
+      { ss. unfold gen_function, type_of_function. ss. rewrite WFMAINSIG in *. ss. }
+    - ss.
+  Qed.
 
 
-
-
-
-
-
-Variant ir_initial_state (p : Asm.program) : ir_state -> Prop :=
-    ir_initial_state_intro : forall (cur : block) (m0 : mem),
-                             let ge := Genv.globalenv p in
-                             Genv.find_symbol ge (AST.prog_main p) = Some cur ->
-                             (exists f : Asm.function, Genv.find_funct_ptr ge cur = Some (AST.Internal f)) ->
-                             Genv.init_mem p = Some m0 -> ir_initial_state p (Some (cur, m0, [])).
-Inductive initial_state (p: program): state -> Prop :=
-  | initial_state_intro: forall b f m0,
-      let ge := Genv.globalenv p in
-      Genv.init_mem p = Some m0 ->
-      Genv.find_symbol ge p.(prog_main) = Some b ->
-      Genv.find_funct_ptr ge b = Some f ->
-      type_of_fundef f = Tfunction Tnil type_int32s cc_default ->
-      initial_state p (Callstate f nil Kstop m0).
-  Definition wf_c_state (ge: Clight.genv) (tr ttr: bundle_trace) (cnts: cnt_ids) id (cst: Clight.state) :=
-    match cst with
-    | State f stmt k_c e le m_c =>
-        wf_counters ge m_c tr cnts /\
-          (exists m_c', Mem.free_list m_c (blocks_of_env ge e) (comp_of f) = Some m_c' /\ wf_c_cont ge m_c' k_c) /\
-          wf_c_stmt ge (comp_of f) cnts id ttr stmt /\
-          (wf_env ge e /\ (not_global_blks (ge) (blocks_of_env2 ge e)) /\ (wf_c_nb ge m_c))
-    | _ => False
-    end.
-  Definition match_state (ge_i: Asm.genv) (ge_c: Clight.genv) (k: meminj) tr cnts pars id (ist: ir_state) (cst: Clight.state) :=
-    match ist, cst with
-    | Some (cur, m_i, k_i), State f _ k_c e le m_c =>
-        (match_genv ge_i ge_c) /\ (match_mem ge_i k m_i m_c) /\
-          (match_cur_fun ge_i ge_c cur f id) /\ (match_find_def ge_i ge_c cnts pars tr) /\
-          (match_cont ge_c tr cnts k_c k_i) /\
-          (match_params pars ge_c ge_i) /\
-          (match_cnts cnts ge_c k)
-    | _, _ => False
-    end.
 
 
 
@@ -914,6 +869,17 @@ Inductive initial_state (p: program): state -> Prop :=
   Definition clight_program_does_prefix (p: Clight.program) (t: trace) :=
     semantics_has_initial_trace_prefix (Clight.semantics1 p) t.
 
+  Lemma star_state_behaves_cut
+        p s0 tr
+        (CUT: exists s1, star step1 (globalenv p) s0 E0 s1 /\
+                      (exists s2 beh, star step1 (globalenv p) s1 tr s2 /\
+                                   state_behaves (semantics1 p) s2 beh))
+    :
+    exists s2 beh, star step1 (globalenv p) s0 tr s2 /\ state_behaves (semantics1 p) s2 beh.
+  Proof.
+    des. exists s2, beh. split; auto. eapply star_trans. 2: eauto. eauto. ss.
+  Qed.
+
   Theorem asm_to_clight
           (p: Asm.program) (ast: Asm.state)
           (WFP: wf_program p)
@@ -921,7 +887,6 @@ Inductive initial_state (p: program): state -> Prop :=
           (WFMAIN: wf_main p)
           (WFMAINSIG: wf_main_sig p)
           (WFINIT: exists (s : Asm.state), Asm.initial_state p s)
-    (* (WF: exists (s: Smallstep.state (semantics p)), Smallstep.initial_state (semantics p) s) *)
     :
     forall tr, asm_program_does_prefix p tr ->
           exists btr,
@@ -944,94 +909,65 @@ Inductive initial_state (p: program): state -> Prop :=
     { eapply MS_I. }
     intros (btr & ist' & UTR & ISTAR). esplits. 2: eauto.
     eapply semantics_has_initial_trace_cut_implies_prefix.
-    assert (INIT_C: exists cst, Clight.initial_state (gen_program btr p) cst).
-    { admit. }
-    des. hexploit ir_to_clight.
+    hexploit exists_initial_state; eauto. instantiate (1:=btr).
+    intros (f_cur & m_c & INIT_C & F_MAIN).
+    (* dup INIT_C. inv INIT_C0. econs 1; ss. eapply INIT_C. eapply star_state_behaves_cut. *)
+    econs 1; ss. eapply INIT_C. eapply star_state_behaves_cut.
+    eexists. split.
+    { econs 2. 2: econs 1. 2: traceEq. eapply step_internal_function.
+      instantiate (3:=empty_env). instantiate (2:=@PTree.empty _). instantiate (1:=m_c).
+      des. econs; ss. all: try rewrite F_MAIN; try rewrite F_MAIN0; try rewrite F_MAIN1; ss.
+      econs. econs. econs.
+    }
+    clear dependent s. clear dependent s'. clear dependent m0. clear beh' j.
+    (* clear - ISTAR INIT_C INIT_MEM_A IR_INIT WFP WFPP WFMAIN WFMAINSIG UTR. *)
+    inv IR_INIT. clarify. des. inv INIT_C. rewrite gen_program_prog_main_eq in *.
+    remember (AST.prog_main p) as id_cur. clear Heqid_cur.
+    hexploit gen_program_match_find_def; eauto. intros MFD.
+    hexploit Genv.find_invert_symbol. eapply H. intros INV_A.
+    dup H0. rewrite Genv.find_funct_ptr_iff in H2. specialize (MFD _ _ _ H2 INV_A).
+    des_ifs. rename Heq into CNT_CUR. rename Heq0 into PAR_CUR.
+    assert (b = cur).
+    { eapply gen_program_symbs_find in H; eauto. ss.
+      subst ge0. setoid_rewrite H5 in H. clarify. ss.
+    }
+    subst b. ss. rewrite <- Genv.find_funct_ptr_iff in MFD.
+    assert (f_cur = (gen_function (Genv.globalenv p) i l (get_id_tr btr id_cur) f)).
+    { subst ge0. setoid_rewrite H6 in MFD. clarify. }
+    clear MFD.
+    hexploit gen_program_match_genv; eauto. instantiate (1:=btr). intros MGENV.
+
+    hexploit ir_to_clight.
     { eapply wf_program_wf_ge; eauto. }
     4: eapply ISTAR.
-    { admit. }
-    { admit. }
-    { admit. }
-    intros CSTAR. des. econs 1; ss.
-    { admit. }
-    hexploit state_behaves_exists. intros (beh2 & BEH2).
-    esplits.
-    { admit. }
-    { eapply BEH2. }
-
-  Admitted.
+    { admit. (* use ISTAR, UTR *) }
+    { instantiate (1:=State f_cur (fn_body f_cur) Kstop empty_env (PTree.empty val) m_c).
+      instantiate (1:=id_cur).
+      instantiate (1:=(get_cnt_ids (gen_counter_defs (next_id (AST.prog_defs p)) (AST.prog_defs p)))).
+      instantiate (1:= globalenv (gen_program btr p)). ss. splits.
+      - admit.
+      - esplits; eauto. econs.
+      - unfold wf_c_stmt. i. subst f_cur. ss. rewrite CNT_CUR in H8. clarify.
+        replace (comp_of (gen_function (Genv.globalenv p) cnt [] (get_id_tr btr id_cur) f)) with
+          (Asm.fn_comp f).
+        2:{ ss. }
+        apply match_symbs_code_bundle_trace. apply MGENV.
+      - ii. des_ifs.
+      - unfold not_global_blks. unfold empty_env. ss. unfold blocks_of_env2, blocks_of_env. ss.
+      - unfold wf_c_nb. ss. erewrite Genv.init_mem_genv_next. reflexivity. auto.
+    }
+    { instantiate (1:= gen_params (next_id (map snd (PTree.elements (gen_counter_defs (next_id (AST.prog_defs p)) (AST.prog_defs p))))) (AST.prog_defs p)).
+      ss. splits.
+      - auto.
+      - admit.
+      - unfold match_cur_fun. ss. splits; ss. eauto.
+      - eapply gen_program_match_find_def; eauto.
+      - econs; auto.
+      - admit.
+      - admit.
+    }
+    intros (cst' & STAR_C). hexploit state_behaves_exists. intros (beh2 & BEH2).
+    esplits; eauto.
   Qed.
-
-    TODO
-
-    Lemma gen_program_exists_initial_state
-          (p: Asm.program) btr
-  (ist : ir_state)
-  (IR_INIT : ir_initial_state p ist)
-      :
-      
-
-(* state_behaves_exists: forall (L : Smallstep.semantics) (s : Smallstep.state L), exists beh : program_behavior, state_behaves L s beh *)
-Inductive initial_state (p: program): state -> Prop :=
-  | initial_state_intro: forall b f m0,
-      let ge := Genv.globalenv p in
-      Genv.init_mem p = Some m0 ->
-      Genv.find_symbol ge p.(prog_main) = Some b ->
-      Genv.find_funct_ptr ge b = Some f ->
-      type_of_fundef f = Tfunction Tnil type_int32s cc_default ->
-      initial_state p (Callstate f nil Kstop m0).
-  Definition wf_c_state (ge: Clight.genv) (tr ttr: bundle_trace) (cnts: cnt_ids) id (cst: Clight.state) :=
-    match cst with
-    | State f stmt k_c e le m_c =>
-        wf_counters ge m_c tr cnts /\
-          (exists m_c', Mem.free_list m_c (blocks_of_env ge e) (comp_of f) = Some m_c' /\ wf_c_cont ge m_c' k_c) /\
-          wf_c_stmt ge (comp_of f) cnts id ttr stmt /\
-          (wf_env ge e /\ (not_global_blks (ge) (blocks_of_env2 ge e)) /\ (wf_c_nb ge m_c))
-    | _ => False
-    end.
-  Definition match_state (ge_i: Asm.genv) (ge_c: Clight.genv) (k: meminj) tr cnts pars id (ist: ir_state) (cst: Clight.state) :=
-    match ist, cst with
-    | Some (cur, m_i, k_i), State f _ k_c e le m_c =>
-        (match_genv ge_i ge_c) /\ (match_mem ge_i k m_i m_c) /\
-          (match_cur_fun ge_i ge_c cur f id) /\ (match_find_def ge_i ge_c cnts pars tr) /\
-          (match_cont ge_c tr cnts k_c k_i) /\
-          (match_params pars ge_c ge_i) /\
-          (match_cnts cnts ge_c k)
-    | _, _ => False
-    end.
-
-Variant ir_initial_state (p : Asm.program) : ir_state -> Prop :=
-    ir_initial_state_intro : forall (cur : block) (m0 : mem),
-                             let ge := Genv.globalenv p in
-                             Genv.find_symbol ge (AST.prog_main p) = Some cur ->
-                             (exists f : Asm.function, Genv.find_funct_ptr ge cur = Some (AST.Internal f)) ->
-                             Genv.init_mem p = Some m0 -> ir_initial_state p (Some (cur, m0, [])).
-   Theorem ir_to_clight
-          (ge_i: Asm.genv) (ge_c: Clight.genv)
-          (WFGE: wf_ge ge_i)
-          ist cst
-          ttr cnts pars k id
-          (BOUND: Z.of_nat (Datatypes.length ttr) < Int64.modulus)
-          (WFC: wf_c_state ge_c [] ttr cnts id cst)
-          (MS: match_state ge_i ge_c k ttr cnts pars id ist cst)
-          ist'
-          (STAR: istar (ir_step) ge_i ist ttr ist')
-    :
-    exists cst', star step1 ge_c cst (unbundle_trace ttr) cst'.
-
-
-
-| step_internal_function : forall (f : function) (vargs : list val) (k : cont) (m : mem) (e : env) (le : temp_env) (m1 : mem),
-                             function_entry f vargs m e le m1 ->
-                             step ge function_entry (Callstate (Internal f) vargs k m) E0 (State f (fn_body f) k e le m1)
-Inductive function_entry1 (ge : genv) (f : function) (vargs : list val) (m : mem) (e : env) (le : temp_env) (m' : mem) : Prop :=
-    function_entry1_intro : forall m1 : mem,
-                            list_norepet (var_names (fn_params f) ++ var_names (fn_vars f)) ->
-                            alloc_variables ge (comp_of f) empty_env m (fn_params f ++ fn_vars f) e m1 ->
-                            bind_parameters ge (comp_of f) e m1 (fn_params f) vargs m' ->
-                            le = create_undef_temps (fn_temps f) -> function_entry1 ge f vargs m e le m'.
-Complements.clight_program_has_initial_trace = 
-fun (p : program) (t : trace) => forall beh : program_behavior, program_behaves (semantics1 p) beh -> behavior_prefix t beh
-     : program -> trace -> Prop
 
 End PROOFINIT.
